RewBasics.ec
@@ -12,7 +12,7 @@ axiom unpair_pair x : unpair (pair_sbits x) = x.
 
 module type Rew = {
   proc getState() : sbits
-  proc * setState(b : sbits) : unit
+  proc setState(b : sbits) : unit
 }.
 
 
@@ -23,7 +23,7 @@ module type Initializer = {
 
 module type RewRun = {
   proc getState() : sbits
-  proc * setState(b : sbits) : unit 
+  proc setState(b : sbits) : unit 
   proc run(z : iat2) : rrt
 }.
 
@@ -37,17 +37,25 @@ module Run(A : RewRun) = {
   proc main(z : iat2) = {
     var r;
     Skip.main();
-    r <- A.run(z);
+    r <@ A.run(z);
     return r;
   }
 }.
 
 
 module GetRunSet(A : RewRun) = {
+  proc getState() = {
+    var s;
+    s <@ A.getState();
+    return s;
+  }
+  proc setState(s : sbits) = {
+    A.setState(s);
+  }
   proc main(z : iat2) = {
     var s , r;
-    s <- A.getState();
-    r <- A.run(z);
+    s <@ A.getState();
+    r <@ A.run(z);
     A.setState(s);
     return r;
   }
@@ -58,7 +66,7 @@ module GetRunSetRun(A : RewRun) = {
   proc main(z : iat2) = {
     var  r;
     GetRunSet(A).main(z);
-    r <- A.run(z);
+    r <@ A.run(z);
     return r;
   }
 }.
@@ -67,18 +75,17 @@ module GetRunSetRunConj(A : RewRun) = {
   module GRS = GetRunSet(A)
   proc main(z : iat2) = {
     var  r1, r2;
-    r1 <- GRS.main(z);
-    r2 <- A.run(z);
+    r1 <@ GRS.main(z);
+    r2 <@ A.run(z);
     return ((z,r1), (z,r2));
   }
 }.
   
 section.
 
+declare module A <: Rew.
 
-declare module A : Rew.
-
-axiom RewProp :
+declare axiom RewProp :
   exists (f : glob A -> sbits),
   injective f /\
   (forall &m, Pr[ A.getState() @ &m : (glob A) = ((glob A){m})
@@ -136,7 +143,7 @@ rewrite ll1.
 have ll3 : forall &m, ((glob A){m} = x)  => Pr[A.getState() @ &m : (glob A) = x /\ res = fA x] = 1%r.
 move => &m eq. byphoare (_: (glob A) = (glob A){m} ==> _) .
 proc*. call (s2 x). auto. auto. auto.
-smt.  
+smt().  
 bypr. progress. apply ll1.
 bypr. rewrite Pr[mu_not]. 
 move => &m e. rewrite (ll2 &m x). auto.
@@ -151,11 +158,11 @@ end section.
 
 section.
 
-declare module A : RewRun.
+declare module A <: RewRun.
 
 
 (* getState lossless follows from rewindable_A, but setState lossless does not, so we ask it *)
-axiom RewProp :
+declare axiom RewProp :
   exists (f : glob A -> sbits),
   injective f /\
   (forall &m, Pr[ A.getState() @ &m : (glob A) = ((glob A){m})
@@ -179,7 +186,7 @@ local lemma GetRunSetRew' : forall (x : (glob A)),
          /\ (glob A){1} = (glob A){2} ==> ={glob A} ].
 move => x rll.
 proc.
-elim (rewindable_A A RewProp).
+elim (rewindable_A A RewProp). 
 move => fA [s1 [s2 [s3]]] s4.
 seq 0 1 : (={glob A} /\ fA x = s{2} /\ fA (glob A){2} = s{2} /\ x{2} = (glob A){2}).
 call{2} (s2 x).
@@ -192,7 +199,7 @@ skip. progress.
 qed.
 
 
-local lemma GetRunSetRew : 
+lemma GetRunSetRew : 
     islossless A.run => 
    equiv [ Skip.main ~ GetRunSet(A).main : ={glob A} ==> ={glob A} ].
 proof. move => ill. 
@@ -218,6 +225,27 @@ skip. by auto.
 qed.
 
 
+lemma GetRunSetRewRes :
+   islossless A.run =>
+  equiv [ A.run ~ GetRunSet(A).main : ={arg, glob A}
+        ==> ={res} ].
+proof.  move => ill.
+  proc*. inline*.
+elim (rewindable_A_plus A RewProp).
+move => fA [s1 [s2 [s2h [s2ll [s3 [s3h ]]]] ]] s3ll.
+sp. wp.
+exists* (glob A){2}. elim*.
+auto.
+seq 0 1 : (A_R = (glob A){2} /\ z0{2} = z{2} /\ ={z, glob A} /\ s{2} = fA A_R).
+
+call {2} (s2 A_R). skip. progress.
+conseq (_: z{1} = z0{2} /\ ={glob A} /\ s{2} = fA A_R  ==> _).  auto.
+seq 1 1 : (r{1} = r0{2} /\ ={glob A} /\ s{2} = fA A_R).
+call (_:true). skip. progress. 
+call {2} (s3 A_R). skip. progress.
+qed.
+
+
 (*  Double run and the respective probabilities: 
 
  forall &m, if   Pr[ A.run @ &m : r ] = p then
@@ -228,7 +256,7 @@ qed.
 
 *)
 
-local lemma dbl1 M : forall (ga : glob A),  forall (p : real),
+lemma dbl1 M : forall (ga : glob A),  forall (p : real),
        phoare[ A.run : (glob A) = ga ==> M res ] = p
     => phoare[ GetRunSet(A).main : (glob A) = ga ==> M res /\ (glob A) = ga ] = p.
 proof.  move => ga p ph. 
@@ -242,7 +270,7 @@ call ph.
 call (s2 ga). skip.  auto.
 call (s3 ga). skip. auto.
 hoare.
-call (_:true). skip. progress. smt.
+call (_:true). skip. progress. smt().
 auto. 
 qed.
 
@@ -261,7 +289,7 @@ call ph.
 call (s2 ga). skip. auto.
 call (s3 ga). skip. auto.
 hoare.
-call (_:true). skip. progress.  smt.
+call (_:true). skip. progress. smt().
 qed.
 
     
@@ -285,7 +313,7 @@ auto.
 skip.   auto.
 hoare.
 call (_:true).
-auto. smt.
+auto. smt().
 auto.
 auto.
 auto.
