RewCommutes.ec
@@ -36,7 +36,7 @@ clone import RewBasics as RW with type sbits <- sbits,
 
 module type GenRewEx1Ex2 = {
   proc getState() : sbits
-  proc * setState(b : sbits) : unit 
+  proc setState(b : sbits) : unit  (* EasyCrypt removed support for "proc *" *)
   proc ex1(x1 : at1 * irt) : rt1
   proc ex2(x2 : at2 * irt) : rt2
 }.
@@ -46,16 +46,16 @@ module ModComm(A : GenRewEx1Ex2, B : Initializer) = {
 
   proc ex2(i12 : at1 * at2,r0 : irt) = {
     var r1, r2,s;
-    s <- A.getState();
-    r1 <- A.ex1(i12.`1,r0);
+    s <@ A.getState();
+    r1 <@ A.ex1(i12.`1,r0);
     A.setState(s);
-    r2 <- A.ex2(i12.`2,r0);
+    r2 <@ A.ex2(i12.`2,r0);
     return (r1,r2);
   }
 
   proc ex1(i0 : iat) = {
     var r0;
-    r0 <- B.init(i0);
+    r0 <@ B.init(i0);
     return r0;
   }
 }.
@@ -63,16 +63,16 @@ module ModComm(A : GenRewEx1Ex2, B : Initializer) = {
 module ModComm'(A : GenRewEx1Ex2, B : Initializer) = {
   proc ex2(i12 : at1 * at2,r0 : irt) = {
     var r1, r2,s;
-    s <- A.getState();
-    r2 <- A.ex2(i12.`2,r0);
+    s <@ A.getState();
+    r2 <@ A.ex2(i12.`2,r0);
     A.setState(s);
-    r1 <- A.ex1(i12.`1,r0);
+    r1 <@ A.ex1(i12.`1,r0);
     return (r1,r2);
   }
 
   proc ex1(i0 : iat) = {
     var r0;
-    r0 <- B.init(i0);
+    r0 <@ B.init(i0);
     return r0;
   }
 }.
@@ -80,12 +80,12 @@ module ModComm'(A : GenRewEx1Ex2, B : Initializer) = {
 
 
 section.
-declare module A : GenRewEx1Ex2.
-declare module B : Initializer.
+declare module A <: GenRewEx1Ex2.
+declare module B <: Initializer.
 
-axiom Bsens : equiv[ B.init ~ B.init : ={arg, glob A, glob B} ==> ={glob A, glob B,res}  ].    
+declare axiom Bsens : equiv[ B.init ~ B.init : ={arg, glob A, glob B} ==> ={glob A, glob B,res}  ].    
 
-axiom RewProp :
+declare axiom RewProp :
   exists (f : glob A -> sbits),
   injective f /\
   (forall &m, Pr[ A.getState() @ &m : (glob A) = ((glob A){m})
@@ -129,7 +129,7 @@ progress.
 exists D.
 exists Q.
 progress. rewrite (H0 (fun r => M )). auto. rewrite - H1.
-rewrite Pr[mu_eq]. smt. auto.
+rewrite Pr[mu_eq]. smt(). auto.
 qed.
 
 
@@ -148,7 +148,7 @@ proof.
 elim (reflectionComp_dmap (ModComm'(A,B))).
 progress.
 exists D. exists Q.
-progress. rewrite (H0 (fun r => M )). auto. rewrite - H1. rewrite Pr[mu_eq]. smt. auto.
+progress. rewrite (H0 (fun r => M )). auto. rewrite - H1. rewrite Pr[mu_eq]. smt(). auto.
 qed.
 
 
@@ -162,11 +162,11 @@ elim reflectionComp2.
 progress. 
 have e1 : Pr[RCR(ModComm'(A, B)).main(i1, i2) @ &m : M res] = 
      Pr[RCR(ModComm'(A, B)).main(i1, i2) @ &m : M (res.`1, (res.`2.`1, res.`2.`2))]. 
-rewrite Pr[mu_eq]. smt. auto.
+rewrite Pr[mu_eq]. smt(). auto.
 rewrite e1.
 have e2 : Pr[RCR(ModComm(A, B)).main(i1, i2) @ &m : M res] = 
      Pr[RCR(ModComm(A, B)).main(i1, i2) @ &m : M (res.`1, (res.`2.`1, res.`2.`2))].
-rewrite Pr[mu_eq]. smt. auto.
+rewrite Pr[mu_eq]. smt(). auto.
 rewrite e2.
 rewrite (H1 &m M').
 rewrite (H4 &m M'  ).  
@@ -192,11 +192,11 @@ rewrite H2.
 simplify pred1.
 have jj : Pr[ModComm'(A,B).ex1(i1) @ &m : (res, ((glob B), (glob A))) = a]
  = Pr[ModComm'(A,B).ex1(i1) @ &m : (res, ((glob B), (glob A))) = a /\ exists &n, (glob B, glob A){n} = a.`2].
-rewrite Pr[mu_eq]. smt.
+rewrite Pr[mu_eq]. smt().
 auto. 
 have yy : Pr[ModComm(A,B).ex1(i1) @ &m : (res, ((glob B), (glob A))) = a]
  = Pr[ModComm(A,B).ex1(i1) @ &m : (res, ((glob B), (glob A))) = a /\ exists &n, (glob B, glob A){n} = a.`2].
-rewrite Pr[mu_eq]. smt.
+rewrite Pr[mu_eq]. smt().
 auto.
 case (! exists &n, (glob B, glob A){n} = a.`2).
 simplify.
@@ -209,7 +209,7 @@ have eq : Pr[ModComm'(A,B).ex1(i1) @ &m :
   have eq1 : Pr[ModComm'(A,B).ex1(i1) @ &m :
    (res, ((glob B), (glob A))) = a /\
    exists &n, ((glob B){n}, (glob A){n}) = a.`2] =  Pr[ModComm'(A,B).ex1(i1) @ &m : false ].
-   rewrite Pr[mu_eq]. smt. auto.
+   rewrite Pr[mu_eq]. smt(). auto.
    rewrite eq1. rewrite Pr[mu_false]. auto. rewrite eq. simplify. clear eq.
 have eq : Pr[ModComm(A,B).ex1(i1) @ &m :
    (res, ((glob B), (glob A))) = a /\
@@ -217,11 +217,11 @@ have eq : Pr[ModComm(A,B).ex1(i1) @ &m :
   have eq1 : Pr[ModComm(A,B).ex1(i1) @ &m :
    (res, ((glob B), (glob A))) = a /\
    exists &n, ((glob B){n}, (glob A){n}) = a.`2] =  Pr[ModComm(A,B).ex1(i1) @ &m : false ].
-   rewrite Pr[mu_eq]. smt. auto.
+   rewrite Pr[mu_eq]. smt(). auto.
    rewrite eq1. rewrite Pr[mu_false]. auto. rewrite eq. simplify. clear eq.
 auto. simplify. move => zzz.
 elim zzz. move => &n np .
-have aa :  a = (a.`1, a.`2). smt.
+have aa :  a = (a.`1, a.`2). smt().
 rewrite aa.
 rewrite - np.
 rewrite - dmeq. rewrite - dmeq.
@@ -234,7 +234,7 @@ have myeq1 : Pr[ModComm'(A,B).ex1(i1) @ &m :
  = Pr[ModComm(A,B).ex1(i1) @ &m :
    (res, ((glob B), (glob A))) = (a.`1, ((glob B){n}, (glob A){n}))].
 byequiv (_: (={arg, glob A, glob B}) ==> ={glob A, glob B,res}).
-proc.  call Bsens. skip. progress. auto. smt. 
+proc.  call Bsens. skip. progress. auto. smt(). 
 rewrite myeq1.
 simplify.
 have q : Pr[ModComm'(A,B).ex2(i2, a.`1) @ &n : M' (a.`1, (res, ((glob B), (glob A))))]
@@ -244,7 +244,7 @@ have q : Pr[ModComm'(A,B).ex2(i2, a.`1) @ &n : M' (a.`1, (res, ((glob B), (glob 
   rewrite Pr[mu_eq]. auto. auto.
   rewrite trv. clear trv.
   byequiv. proc. call (_:true). call (_:true). call (_:true). call(_:true).
-  skip. progress. smt. auto. 
+  skip. progress. smt(). auto. 
 rewrite q. clear q.
 have q : Pr[ModComm(A,B).ex2(i2, a.`1) @ &n : M' (a.`1, (res, ((glob B), (glob A))))]
  =    Pr[CommNoInit(A).ex1ex2((i2.`1, a.`1), (i2.`2 , a.`1)) @ &n : M (a.`1, res)].
@@ -253,11 +253,11 @@ have q : Pr[ModComm(A,B).ex2(i2, a.`1) @ &n : M' (a.`1, (res, ((glob B), (glob A
   rewrite Pr[mu_eq]. auto. auto.
   rewrite trv. clear trv.
   byequiv. proc. call (_:true). call (_:true). call (_:true). call(_:true).
-  skip. progress. smt. auto. 
+  skip. progress. smt(). auto. 
 rewrite q. clear q.
 have q : Pr[CommNoInit(A).ex1ex2((i2.`1, a.`1), (i2.`2, a.`1)   ) @ &n : M (a.`1, res)] 
   = Pr[CommNoInit(A).ex2ex1((i2.`1, a.`1), (i2.`2, a.`1)) @ &n : M (a.`1, res)].
-  have kk : i2 = (i2.`1, i2.`2). smt.
+  have kk : i2 = (i2.`1, i2.`2). smt().
   rewrite kk.
  apply (rew_comm_law_simple A RewProp &n 
          (fun (x : rt1 * rt2) => M (a.`1, x)) 
@@ -292,7 +292,11 @@ clone import RewBasics as RW with type sbits <- sbits,
                                   type irt <- irt,
                                   type iat <- iat,
                                   op pair_sbits <- pair_sbits,
-                                  op unpair <- unpair.
+                                  op unpair <- unpair
+proof*.
+realize ips. apply ips. qed.
+realize unpair_pair. apply unpair_pair. qed.
+
 
 
 clone import GenRewCommutes as GRC with type at1 <- unit,
@@ -309,7 +313,7 @@ clone import GenRewCommutes as GRC with type at1 <- unit,
 
 module type SpecRewEx1Ex2 = {
   proc getState() : sbits
-  proc * setState(b : sbits) : unit 
+  proc setState(b : sbits) : unit (* EasyCrypt removed support for "proc *" *)
   proc ex1(x1 : irt) : rt1
   proc ex2(x2 : irt) : rt2
 }.
@@ -318,35 +322,35 @@ module type SpecRewEx1Ex2 = {
 module SpecRewComm(A : SpecRewEx1Ex2, B : Initializer) = {
   proc iex1ex2(i0 : iat) = {
     var r0, r1, r2, s;
-    r0 <- B.init(i0);
-    s <- A.getState();
-    r1 <- A.ex1(r0);
+    r0 <@ B.init(i0);
+    s <@ A.getState();
+    r1 <@ A.ex1(r0);
     A.setState(s);
-    r2 <- A.ex2(r0);
+    r2 <@ A.ex2(r0);
     return (r0, (r1, r2));
   }
 
   proc iex2ex1(i0 : iat) = {
     var r0, r1, r2, s;
-    r0 <- B.init(i0);
-    s <- A.getState();
-    r2 <- A.ex2(r0);
+    r0 <@ B.init(i0);
+    s <@ A.getState();
+    r2 <@ A.ex2(r0);
     A.setState(s);
-    r1 <- A.ex1(r0);
+    r1 <@ A.ex1(r0);
     return (r0, (r1, r2));
   }
 }.
 
 
 section.
-declare module A : SpecRewEx1Ex2.
-declare module B : Initializer.
+declare module A <: SpecRewEx1Ex2.
+declare module B <: Initializer.
 
 
 local module WA = {
   proc getState() : sbits = {
     var r;
-    r <- A.getState();
+    r <@ A.getState();
     return r;
   }
   proc setState(b : sbits) : unit  = {
@@ -354,21 +358,21 @@ local module WA = {
   }
   proc ex1(x1 : unit * irt) : rt1 = {
     var r;
-    r <- A.ex1(x1.`2);
+    r <@ A.ex1(x1.`2);
     return r;
   }
   proc ex2(x2 : unit * irt) : rt2 = {
     var r;
-    r <- A.ex2(x2.`2);
+    r <@ A.ex2(x2.`2);
     return r;
   }
 }.
 
 
-axiom Bsens : equiv[ B.init ~ B.init : ={arg, glob A, glob B} ==> ={glob A, glob B,res}  ].
+declare axiom Bsens : equiv[ B.init ~ B.init : ={arg, glob A, glob B} ==> ={glob A, glob B,res}  ].
 
 
-axiom RewProp :
+declare axiom RewProp :
   exists (f : glob A -> sbits),
   injective f /\
   (forall &m, Pr[ A.getState() @ &m : (glob A) = ((glob A){m})
@@ -391,7 +395,7 @@ skip.  progress.
 seq 1 1 : (={glob A, glob B, r0}). call Bsens. skip. progress. 
 wp.  sp.
 call (_:true). wp. call (_:true).  wp.  call (_:true). wp.  call (_:true). skip. progress.
-smt. auto. 
+smt(). auto. 
 rewrite (eq (tt, tt)). clear eq. 
 have eq : forall i2, Pr[SpecRewComm(A, B).iex2ex1(i0) @ &m : M res] =
    Pr[RC.RCR(ModComm'(WA, B)).main(i0, i2) @ &m : M res].
@@ -402,19 +406,19 @@ skip. progress.
 seq 1 1 : (={glob A, glob B, r0}). call Bsens. skip. progress. 
 wp.  sp.
 call (_:true). wp. call (_:true). wp. call (_:true). wp. call (_:true). skip. progress.
-smt. auto. 
+smt(). auto. 
 rewrite (eq (tt, tt)). clear eq. 
-rewrite (reflectionComb WA B).
-simplify. apply Bsens. 
+rewrite (reflectionComb WA B). auto.
+simplify. apply Bsens.
 simplify.
-elim (rewindable_A A RewProp). progress. 
-     exists f. progress.  
-byphoare (_: (glob A) = (glob A){m0} ==> _).   
+elim (rewindable_A A RewProp). progress.
+     exists f. progress.
+byphoare (_: (glob A) = (glob A){m0} ==> _).
      proc. call (H0 (glob A){m0}). skip. auto. auto. auto.
-byphoare (_: arg = f x /\ (glob A) = (glob A){m0}  ==> _).      
+byphoare (_: arg = f x /\ (glob A) = (glob A){m0}  ==> _).
 proc. call (H1 x). skip. auto. progress.  auto.
-proc. call H2. skip. auto.
-apply ips. apply unpair_pair. apply ips. apply unpair_pair. auto.
+proc. call H2. skip. auto. auto.
+(* apply ips. apply unpair_pair. apply ips. apply unpair_pair. auto. *)
 qed.
 
 
