JensensInf.ec
@@ -23,41 +23,47 @@ proof. progress.
 elim (fin_pr_approx_distr X).
 move => J [Je Jp].
 have edc : 0%r < (epsilon / (d - c)).
-smt.
+smt().
 elim (Jp (epsilon / (d - c))  edc ).
 move => N Np. 
 exists (mem ((pmap J ((range 0 N))))).
 split. 
 apply mkfinite. exists (pmap J (range 0 N)).
 auto.
-smt.
+smt().
 qed.
 
 
 local lemma is_loss ['a] (X : 'a distr) M : mu X M > 0%r 
  => is_lossless (inv (mu X M)  \cdot drestrict X M).
-proof. have dw : weight (drestrict X M) = (mu X M). smt.
+proof. have dw : weight (drestrict X M) = (mu X M). smt(@Distr).
 rewrite - dw.
 apply dscalar_ll.
 qed.
 
 
+
+local lemma has_E' k (X : 'a distr) g :  hasE X g  => 0%r <= k && k <= inv (weight X)
+ => hasE (k \cdot X) g.
+rewrite /hasE. progress.
+
+have ->: (fun (x : 'a) => g x * mu1 (k \cdot X) x)
+ = (fun (x : 'a) => k * (g x * mu1 X x)).
+apply fun_ext. move => x. rewrite dscalar1E. auto.
+auto. smt().
+apply summableZ. auto.
+qed.
+
+
 local lemma has_E (X : 'a distr) M g :  mu X M > 0%r => hasE X g 
  => hasE (inv (mu X M) \cdot drestrict X M) g.
-proof.  move => mpos he.
-rewrite /hasE.
-  have ->: (fun (x : 'a) => g x * mass (inv (mu X M) \cdot drestrict X M) x)
-      =  (fun (x : 'a) => g x * inv (mu X M) * mass (drestrict X M) x).
-  apply fun_ext.
-  move => x.
-  rewrite massE.
-  rewrite dscalar1E. split. smt.  move => p.
-  have ->: mu X M = weight (drestrict X M). timeout 20. smt.
-  auto. smt.
-  have : hasE (drestrict X M) (fun x => inv (mu X M) * g x).
-  apply hasEZ. smt.
-rewrite /hasE.
-simplify. auto.
+proof. progress.
+have f1 : hasE (drestrict X M) g. 
+apply hasE_drestrict. auto.
+apply has_E'. auto.
+split. smt(). progress.
+have ->: (weight (drestrict X M)) = mu X M. smt(@Distr).
+auto.
 qed.
 
 
@@ -71,18 +77,42 @@ rewrite /(dscalar).
     rewrite /mscalar.
 have ss : isdistr (fun (x0 : 'a) => c * mass X x0).
 apply isdistr_mscalar.
-smt.
-smt. smt.
+have ->: (fun (x0 : 'a) => mass X x0) = (fun (x0 : 'a) => mu1 X x0). apply fun_ext. smt(massE).
+apply isdistr_mu1. 
+split.
+smt().
+progress. 
+rewrite weightE.
+have ->: (fun (x0 : 'a) => mu1 (mk (mass X)) x0)
+ = (fun (x0 : 'a) => mu1 X x0).
+apply fun_ext. move => x0. 
+rewrite  muK. 
+have ->: (mass X) = mu1 X. smt(massE).
+apply isdistr_mu1. 
+smt(massE).
+rewrite - weightE. smt().
+rewrite muK. 
+apply isdistr_mscalar. apply isdistr_mu1.
+split. smt().
+progress.
+have ->: (weight (mk (fun (x0 : 'a) => mu1 X x0)))
+ = weight X.
+rewrite weightE. rewrite weightE. simplify.
+have ->: (fun (x0 : 'a) => mu1 (mk (fun (x0_0 : 'a) => mu1 X x0_0)) x0)
+ = (fun (x0 : 'a) => mu1 X x0). apply fun_ext.  move => x0.
+rewrite muK. 
+apply isdistr_mu1. simplify. auto. auto. smt(@Distr).
+smt().
 qed.
 
 
 local lemma www (X : 'a distr) (g : 'a -> real) M: 
  Ec X g M = (inv (mu X M)) * E (drestrict X M) g.
-proof. smt. qed.
-
+proof. smt (@Distr @Real qqq). 
+qed.
 
 local lemma iii a b : (a > 0%r) => (b > 0%r) => b <= a => inv a <= inv b .
-smt.
+smt().
 qed.
 
 
@@ -101,26 +131,34 @@ have s2 : isdistr (fun (x0 : 'a) =>
         inv (mu X M) * (fun (x1 : 'a) => if M x1 then mu1 X x1 else 0%r) x0).
 apply isdistr_mscalar. apply s1.
 split.
-smt.
+smt(@Distr @Real).
 move => q1.
-simplify.
 have ->: mu (mk (fun (x1 : 'a) => if M x1 then mu1 X x1 else 0%r)) predT = mu X M.
 rewrite muE. rewrite muE.
 apply eq_sum.
 move => y. simplify.
 simplify predT.
 rewrite muK. apply s1.
+simplify. auto. auto.
 simplify.
-rewrite massE. auto.
-auto.
-rewrite muK. apply s2.
-smt.
+rewrite muE. 
+have f : (fun (x0 : 'a) =>
+     mu1 (mk (fun (x1 : 'a) => if M x1 then mu1 X x1 else 0%r)) x0 / mu X M)
+ = (fun (x0 : 'a) => (if M x0 then mu1 X x0 else 0%r) / mu X M).
+apply fun_ext. move => x0. rewrite muK. 
+smt(). smt().
+rewrite muK.  rewrite f. smt().
+rewrite f.
+simplify.
+have ->: sum (fun (x0 : 'a) => if pred1 x x0 then mu1 X x0 else 0%r)
+  =  mu1 X x.
+rewrite muE. auto. auto.
 qed.
 
 
 local lemma uuu (X : 'a distr) (g : 'a -> real) M :
   (inv (mu X M)) * E (drestrict X M) g = Ec X g M.
-proof. smt. qed.
+proof. smt(www). qed.
 
 
 local lemma Jensen_inf1 (X : 'a distr) (g : 'a -> real) M:
@@ -133,7 +171,7 @@ qed.
 
 
 local lemma ec_edot (X : 'a distr) M g : Ec X g M = E (inv (mu X M) \cdot drestrict X M) g.
-proof. rewrite - ooo. smt. qed.
+proof. rewrite - ooo. smt(www). qed.
 
 
 local lemma Jensen_inf_1 (X : 'a distr) (g : 'a -> real) M:
@@ -145,10 +183,10 @@ rewrite (Jensen_inf1 X g M). auto.
 rewrite - ooo. rewrite - ooo.
 rewrite exp_drestrict.
 have opp : (inv (mu X M) * (mu X M * Ec X g M)) = Ec X g M.
-smt.
+rewrite - uuu. smt(@Real).
 rewrite opp.
 have ppo : mu X (predC M) * (inv (mu X (predC M)) * E (drestrict X (predC M)) g) =  E (drestrict X (predC M)) g.
-smt.
+smt(@Real @Distr).
 rewrite ppo.
 rewrite exp_drestrict.
 auto.
@@ -162,10 +200,10 @@ local lemma Jensen_inf2 (X : 'a distr) (g : 'a -> real) f M:
     <= mu X M * f (Ec X g M)
     + mu X (predC M) * f (Ec X g (predC M)).
 proof.  move => llX fconv.
-have co : mu X (predC M) = 1%r - mu X M. smt.
+have co : mu X (predC M) = 1%r - mu X M. smt(@Distr).
 rewrite co.
 apply (fconv (Ec X g M) (Ec X g (predC M)) (mu X M)).
-smt.
+smt(@Distr).
 qed.
 
 
@@ -178,8 +216,8 @@ proof.
 move => D g b ll ld he.
 have zz : E D (fun _ => b) <= b.
 rewrite expC.
-have ws1 : weight D <= 1%r. smt.
-have ws2 : 0%r <= weight D. smt. smt.
+have ws1 : weight D <= 1%r. smt().
+have ws2 : 0%r <= weight D. smt(). smt().
 apply (ler_trans (E D (fun (_ : 'a) => b))).
 apply in_ler_exp.
 apply he.
@@ -196,7 +234,7 @@ local lemma Jensen_inf4_gen_2 ['a] : forall D (g : 'a -> real) a,
 move => D g a ld q he.
 have zz : a = E D (fun _ => a).
 rewrite expC.
-smt.
+smt().
 rewrite  zz.
 apply in_ler_exp.
 apply hasEC.
@@ -206,7 +244,7 @@ qed.
 
 
 local lemma wdrestr (X : 'a distr) M : (mu X M) = (weight (drestrict X M)).
-proof. smt. qed.
+proof. smt(@Distr). qed.
 
 
 local lemma jensen_ie (X : 'a distr) g f (a b c d : real) :
@@ -223,53 +261,53 @@ case (b < a). move => p.
 have : exists x, x \in X.
 elim (witness_support  predT X).
 move => i1 _. 
-  have wo : 0%r < weight X. smt.
+  have wo : 0%r < weight X. smt().
   elim (i1 wo).
-smt.
+smt().
 elim. move=> x xi.
 have : false.
-  have : a <= g x.  smt. 
+  have : a <= g x.  smt(). 
   have : a <= g x && g x <= b. apply xvals. apply xi.
   move => [f1 f2]  .
-  have : g x = b. smt.
-  have : g x = a. smt.
-  smt.
-  smt.
+  have : g x = b. smt().
+  have : g x = a. smt().
+  smt().
+  smt().
 move => nabp.
-have abp : a <= b. smt.
+have abp : a <= b. smt().
 case (d < c). move => p.
 have : c <= f a && f a <= d.
-apply fvals. split. smt. move => _. apply abp. 
+apply fvals. split. smt(). move => _. apply abp. 
 move => [f1 f2].
-have : f a = c. smt.
-have : f a = d. smt.
-smt.
+have : f a = c. smt().
+have : f a = d. smt().
+smt().
 case (d = c). move => dce.
 have : forall x, a <= x <= b => c <= f x <= d.
 move => x xp.
 apply (fvals x xp).
 rewrite dce. move => ep.   
 have : forall x, a <= x <= b => f x = c.
-smt.
+smt().
 move => fpv _.
   have : a <= E X g <= b.
    split.     
   have ->: a = E X (fun x => a).
-  rewrite expC. smt.
+  rewrite expC. smt().
   apply in_ler_exp. apply hasEC. apply XghasE.
-  smt.  
+  smt().  
   have ->: b = E X (fun x => b).
-  rewrite expC. smt. move => _.   apply in_ler_exp.  apply XghasE. apply hasEC.
-  smt.    
+  rewrite expC. smt(). move => _.   apply in_ler_exp.  apply XghasE. apply hasEC.
+  smt().    
 move => ei.
-have ->: f (E X g) = c. smt.
-rewrite (eq_exp X (f \o g) (fun _ => c)). smt.
+have ->: f (E X g) = c. smt().
+rewrite (eq_exp X (f \o g) (fun _ => c)). smt().
 have ->: E X (fun (_ : 'a) => c) = c.
-rewrite expC. smt.
-smt. 
+rewrite expC. smt().
+smt(). 
 move => ndcp1 ndcp2.
 have  dcp : c < d.
-smt.
+smt().
 elim (Jensen_inf0 X d c eps  eprop dcp).
 move => M p. elim p.
 move => finM muXC.
@@ -279,7 +317,7 @@ apply (Jensen_inf2 X g f M). auto.  auto. (* step 2 *)
 apply (ler_trans (mu X M *  (Ec X (f \o g) M) + mu X (predC M) * f (Ec X g (predC M)))).
 rewrite ec_edot.
 case ((mu X M) = 0%r).
-smt.
+smt().
 move => mupos.
   have ff1 : f (E (inv (mu X M) \cdot drestrict X M) g)
       <= (E (inv (mu X M) \cdot drestrict X M) (f \o g)).
@@ -289,110 +327,112 @@ have dfin : is_finite (support (inv (mu X M) \cdot drestrict X M)).
    elim finM.
    move => s spr.  exists (filter (fun x => mu1 X x <> 0%r) s).
    rewrite /is_finite_for.
-   split. smt.
+   split. smt(@List).
    move => x.
    split.
    move => xi.
    elim (spr). move => _ pr.
    elim (pr x).      move => p1 p2.
-   have Mx : M x. smt.
-   have xX : x \in X. smt.
-   have xXM : x \in (drestrict X M). smt.
-   apply supp_dscalar. smt.
+   have Mx : M x. smt(@List).
+   have xX : x \in X. smt(@Distr @List).
+   have xXM : x \in (drestrict X M). smt(@Distr).
+   apply supp_dscalar. smt(@Distr).
    have ->: (mu X M) = (weight (drestrict X M)). apply wdrestr.  auto.  auto.
    move => pr.
     have  xiX : forall x, x \in (inv (mu X M) \cdot drestrict X M)
        => x \in (drestrict X M).
        move => y pr1.
        have : y \in (inv (mu X M) \cdot drestrict X M) <=> y \in drestrict X M.
-       apply supp_dscalar. smt.
+       apply supp_dscalar. smt(@Distr).
        have : weight (drestrict X M) = mu X M. rewrite -  wdrestr.  auto.
-       smt. move => eq. smt. 
-       smt.
+       smt(). move => eq. smt(@Distr). 
+       have o1 : x \in s. smt(@Distr).
+       have o2 : mu1 X x <> 0%r. smt(@Distr).
+       smt(@List).
  auto. 
-apply is_loss. smt. apply fconv.
+apply is_loss. smt(@Distr). apply fconv.
   rewrite (ec_edot X M (f \o g)).
   have ff2 : mu X M >= 0%r.
-  smt.
-  smt.        (* step 3 *)
+  smt(@Distr).
+  smt().        (* step 3 *)
 apply (ler_trans
   (mu X M *  (Ec X (f \o g) M) + mu X (predC M) * d)).
 case ((mu X (predC M)) = 0%r).
-smt.
+smt().
 move => nz.
    have ff1 : f (Ec X g (predC M)) <= d.
      have ff2 : a <= Ec X g (predC M) <= b.
       split. rewrite ec_edot. apply Jensen_inf4_gen_2. apply is_loss.
-      smt.
+      smt(@Distr).
 have  xiX : forall x, x \in (inv (mu X (predC M)) \cdot drestrict X (predC M))
    => x \in X.
    move => x pr.
    have : x \in (inv (mu X (predC M)) \cdot drestrict X (predC M)) <=> x \in drestrict X (predC M).
-   apply supp_dscalar. smt.
+   apply supp_dscalar. smt(@Real @Distr).
    have : weight (drestrict X (predC M)) = mu X (predC M).
-   smt. move => eq. smt.
-   smt. smt.
-   apply has_E.        smt. smt. progress. rewrite ec_edot. apply Jensen_inf4_gen_1. smt.
+   smt(@Distr). move => eq. smt().
+   smt(@Distr). smt().
+   apply has_E. smt(@Distr). smt(). progress. rewrite ec_edot. apply Jensen_inf4_gen_1. 
+   apply is_loss. smt(@Distr).
 have  xiX : forall x, x \in (inv (mu X (predC M)) \cdot drestrict X (predC M))
    => x \in X.
    move => x pr.
    have : x \in (inv (mu X (predC M)) \cdot drestrict X (predC M)) <=> x \in drestrict X (predC M).
-   apply supp_dscalar. smt.
+   apply supp_dscalar. smt(@Distr).
    have : weight (drestrict X (predC M)) = mu X (predC M).
-   smt. move => eq. smt.
-   smt. smt.
-apply has_E. smt.
-smt.
+   smt(@Distr). move => eq. smt(@Distr).
+   smt(@Distr). smt().
+apply has_E. smt(@Distr).
+smt().
 have dp : mu X (predC M) * f (Ec X g (predC M)) <= mu X (predC M) * d.
-  have qq : forall (a b c : real), a >= 0%r => b <= c => a * b <= a * c. smt.
-  have mup : mu X (predC M) >= 0%r. smt.
+  have qq : forall (a b c : real), a >= 0%r => b <= c => a * b <= a * c. smt().
+  have mup : mu X (predC M) >= 0%r. smt(@Distr).
   (*have dp  : d >= 0%r. smt. *)
-  smt.
-smt.
-  have mup : mu X (predC M) >= 0%r. smt.
+  smt().
+smt().
+  have mup : mu X (predC M) >= 0%r. smt(@Distr).
   have : mu X (predC M) * f (Ec X g (predC M)) <= mu X (predC M) * d.
-   clear finM muXC nz eprop.  smt.
-  smt.
+   clear finM muXC nz eprop. smt().
+  smt().
 apply (ler_trans (E X (f \o g) -  mu X (predC M) * Ec X (f \o g) (predC M) + mu X (predC M) * d)).
   have : E X (f \o g) = mu X M * Ec X (f \o g) M
                         + mu X (predC M) * Ec X (f \o g) (predC M).
   apply Ec_split. apply XfghasE.
 move => eq.
-   have : mu X (predC M) * Ec X (f \o g) (predC M) =  E X (f \o g) - mu X M * Ec X (f \o g) M. smt.
+   have : mu X (predC M) * Ec X (f \o g) (predC M) =  E X (f \o g) - mu X M * Ec X (f \o g) M. smt().
    move => eq2.  rewrite  eq2.
-   have ->: E X (f \o g) - (E X (f \o g) - mu X M * Ec X (f \o g) M) = mu X M * Ec X (f \o g) M . smt.
+   have ->: E X (f \o g) - (E X (f \o g) - mu X M * Ec X (f \o g) M) = mu X M * Ec X (f \o g) M. smt().
  auto.
 apply (ler_trans (E X (f \o g) -  mu X (predC M) * c + mu X (predC M) * d)).
-   case (mu X (predC M) = 0%r). smt.
+   case (mu X (predC M) = 0%r). smt().
    move => mpMnz.
    have cb : c <= Ec X (f \o g) (predC M).
    rewrite ec_edot.
-   apply (Jensen_inf4_gen_2 (inv (mu X (predC M)) \cdot drestrict X (predC M)) (f \o g) ).  apply is_loss. smt.
+   apply (Jensen_inf4_gen_2 (inv (mu X (predC M)) \cdot drestrict X (predC M)) (f \o g) ).  apply is_loss. smt(@Distr).
 have  xiX : forall x, x \in (inv (mu X (predC M)) \cdot drestrict X (predC M))
    => x \in X.
    move => x pr.
    have : x \in (inv (mu X (predC M)) \cdot drestrict X (predC M)) <=> x \in drestrict X (predC M).
-   apply supp_dscalar. smt.
+   apply supp_dscalar. smt(@Distr).
    have : weight (drestrict X (predC M)) = mu X (predC M).
-   smt. move => eq. smt.
-   smt.
-smt.
- apply has_E. smt. apply XfghasE.
+   smt(@Distr). move => eq. smt().
+   smt(@Distr).
+smt().
+ apply has_E. smt(@Distr). apply XfghasE.
   have : E X (f \o g) - mu X (predC M) * Ec X (f \o g) (predC M) <=
          E X (f \o g) - mu X (predC M) * c.
      have muc : mu X (predC M) * c <= mu X (predC M) * Ec X (f \o g) (predC M).
-      have mup : mu X (predC M) >= 0%r. smt.
-      clear finM muXC eprop.   smt.
-     smt.
-smt.
+      have mup : mu X (predC M) >= 0%r. smt(@Distr).
+      clear finM muXC eprop. smt().
+     smt().
+smt().
 have ->: E X (f \o g) - mu X (predC M) * c + mu X (predC M) * d
   =    E X (f \o g) + (d - c) * mu X (predC M).
-smt.
-(* have dcp : (d - c) >= 0%r. smt. *)
+smt().
 apply (ler_trans (E X (f \o g) + (d - c) *   (eps / (d-c)) )).  clear XghasE XfghasE fconv ll fvals xvals finM.
-   have trivia: forall (a b c : real), a >= 0%r => b <= c => a * b <= a * c. smt.
+   have trivia: forall (a b c : real), a >= 0%r => b <= c => a * b <= a * c. smt().
    have trivia2 : (d - c) * mu X (predC M) <= (d - c) * (eps / (d - c)). apply trivia. auto. auto.
-smt. smt. smt. smt.
+smt(). smt(). smt(). smt().
 qed.
 
 
@@ -408,7 +448,7 @@ proof. progress. apply sm_than.
 progress.
   have sm : f (E X g) <= E X (f \o g) + e.
   apply (jensen_ie X g f a b c d);auto.
-smt.
+smt().
 qed.
 
 
