JensensSquare.ec
@@ -43,10 +43,10 @@ smt. apply square_convex.
 have : forall f, E (dscale d) f = (E d f) / (weight d).
 move => g.
 simplify E.
-have : (fun (x : 'a) => g x * mass (dscale d) x) = (fun (x : 'a) =>  1%r/(weight d) * (g x * mass d x)).
+have : (fun (x : 'a) => g x * mu1 (dscale d) x) = (fun (x : 'a) =>  1%r/(weight d) * (g x * mu1 d x)).
 apply fun_ext. move => x. simplify.
-rewrite massE. smt.
-move =>  k. rewrite k.
+smt.
+move =>  k. rewrite  k.
 rewrite sumZ. smt.
 move => l.
 rewrite (l f).
@@ -66,17 +66,18 @@ qed.
 lemma jen_big ['a] :
   forall (d : 'a distr) (f : 'a -> real) J,
   is_finite (support d) => uniq J =>
-    (forall (x : 'a), (fun (x : 'a) => f x * mass d x) x <> 0%r => x \in J) 
-  => (big predT (fun (x : 'a) => f x * mass d x) J) ^ 2
-    <= (big predT (fun (x : 'a) => square (f x) * mass d x) J).
+    (forall (x : 'a), (fun (x : 'a) => f x * mu1 d x) x <> 0%r => x \in J) 
+  => (big predT (fun (x : 'a) => f x * mu1 d x) J) ^ 2
+    <= (big predT (fun (x : 'a) => square (f x) * mu1 d x) J).
 proof. simplify.
 move => d f J fd uJ pJ1. 
-  have pJ2 : forall (x : 'a), (fun (x0 : 'a) => square (f x0) * mass d x0) x <> 0%r => x \in J.
+  have pJ2 : forall (x : 'a), (fun (x0 : 'a) => square (f x0) * mu1 d x0) x <> 0%r => x \in J.
 auto. move => x. simplify. move => pr. apply pJ1.
-   have : mass d x <> 0%r.  smt.
+   have : mu1 d x <> 0%r.  smt.
    smt.
-rewrite - (sumE_fin (fun (x : 'a) => f x * mass d x) J uJ pJ1). 
-rewrite - (sumE_fin (fun (x : 'a) => square (f x) * mass d x) J uJ pJ2).  
+rewrite - (sumE_fin (fun (x : 'a) => f x * mu1 d x) J uJ pJ1). 
+rewrite - (sumE_fin (fun (x : 'a) => square (f x) * mu1 d x) J uJ pJ2).  
+
 apply Jensen_fin_without_lossless.
 auto.
 qed.
@@ -85,13 +86,13 @@ qed.
 lemma jen_big_spec ['a] :
   forall (d : 'a distr) (f : 'a -> real) J,
   is_finite (support d) => uniq J =>
-    (forall (x : 'a), (fun (x : 'a) => f x * mass d x) x <> 0%r => x \in J) 
-  => (big predT (fun (x : 'a) => mass d x * f x) J) ^ 2
-    <= (big predT (fun (x : 'a) => mass d x * (f x) * (f x)) J).
+    (forall (x : 'a), (fun (x : 'a) => f x * mu1 d x) x <> 0%r => x \in J) 
+  => (big predT (fun (x : 'a) => mu1 d x * f x) J) ^ 2
+    <= (big predT (fun (x : 'a) => mu1 d x * (f x) * (f x)) J).
 proof. progress.
-have : (fun (x : 'a) => mass d x * f x) = (fun (x : 'a) => f x * mass d x).
+have : (fun (x : 'a) => mu1 d x * f x) = (fun (x : 'a) => f x * mu1 d x).
 apply fun_ext. move => x. smt.
-have : (fun (x : 'a) => mass d x * f x * f x) = (fun (x : 'a) => square (f x) * mass d x).
+have : (fun (x : 'a) => mu1 d x * f x * f x) = (fun (x : 'a) => square (f x) * mu1 d x).
 apply fun_ext. move => x. smt.
 move => e1 e2. rewrite e1 e2.
 apply jen_big.
@@ -165,11 +166,11 @@ move => s us.
 have : big predT (fun (x : 'a) => if x \in J then d x else 0%r) s <=  big predT d s .
   apply big_rest_sm. auto. 
 smt.
-have e : (fun (x : 'a) => if x \in J then d x * f x else 0%r) = (fun (x : 'a) => mass (mk (fun x => if x \in J then d x else 0%r)) x * f x ). apply fun_ext.
+have e : (fun (x : 'a) => if x \in J then d x * f x else 0%r) = (fun (x : 'a) => mu1 (mk (fun x => if x \in J then d x else 0%r)) x * f x ). apply fun_ext.
 move => x. simplify.  smt.
 rewrite e. clear e.
 have e : (fun (x : 'a) => if x \in J then d x * f x * f x else 0%r) 
- = (fun (x : 'a) => mass (mk (fun x => if x \in J then d x else 0%r)) x * f x  * f x).
+ = (fun (x : 'a) => mu1 (mk (fun x => if x \in J then d x else 0%r)) x * f x  * f x).
 apply fun_ext. move => x. smt. rewrite e. clear e.
 apply (jen_big_spec (mk (rest d J)) f).
 exists (filter (fun x => d x > 0%r) J). split.
@@ -178,20 +179,18 @@ move => x. split.
 move => xj. simplify rest. 
 have : support (mk (rest d J)) x.
    have : 0%r < d x . smt. move => m0.
-   have : mu (mk (rest d J)) (pred1 x)  = d x. rewrite - massE.
+   have : mu (mk (rest d J)) (pred1 x)  = d x. 
    rewrite muK. auto.  have : x \in J. smt. move => xj'. smt.
    move => m1.
  smt.
 auto.
 move => xmrd. 
 have : (rest d J) x <> 0%r.
-have : (mass (mk (rest d J))) x <> 0%r. smt. 
-rewrite muK. auto. auto.
+have : (mu1 (mk (rest d J))) x <> 0%r. smt. 
+auto. auto.
 move => kll.
-have : d x <> 0%r. smt.
-move => dxo. smt.
-auto.
-simplify.
-move => x. rewrite muK. auto. 
-smt.
+have : d x <> 0%r. smt(muK).
+move => dxo. smt(muK).
+smt. auto. 
+smt(muK).
 qed.
