RandomFacts.ec
@@ -8,6 +8,7 @@ require (*--*) FinType.
 require import Logic.
 
 
+
 (* "sum" interpretation of dlet *)
 lemma dlet_mu_main ['a, 'b]:
   forall (d : 'a distr) (f : 'a -> 'b distr) M,
@@ -17,17 +18,17 @@ have dletE_swap' :
     mu (dlet d f) P = 
     sum (fun (a : 'a) => (mass d a) * 
                           sum (fun (b : 'b) => if P b then  mass (f a) b else 0%r)).
-move => d f P. rewrite dletE_swap.
+move => d f P. rewrite  dlet_muE_swap.
 have qq : (fun (a : 'a) =>
-     sum (fun (b : 'b) => if P b then mass d a * mass (f a) b else 0%r)) 
+     sum (fun (b : 'b) => if P b then mu1 d a * mu1 (f a) b else 0%r)) 
  =  (fun (a : 'a) =>
       sum (fun (b : 'b) => mass d a  * (if P b then mass (f a) b else 0%r))).
 apply fun_ext. move => a. 
-have aux2 : (fun (b : 'b) => if P b then mass d a * mass (f a) b else 0%r)  
+have aux2 : (fun (b : 'b) => if P b then mu1 d a * mu1 (f a) b else 0%r)  
  = (fun (b : 'b) => mass d a * if P b then mass (f a) b else 0%r). 
-apply fun_ext. move => b. smt.
+apply fun_ext. move => b. smt(massE).
 rewrite aux2. auto.
-rewrite qq.
+rewrite  qq.
 have aux3 : (fun (a : 'a) =>
      sum (fun (b : 'b) => mass d a * if P b then mass (f a) b else 0%r)) = 
       (fun (a : 'a) =>
@@ -40,53 +41,50 @@ have qqq : (fun (a : 'a) => mu1 d a * mu (f a) M) = (fun (a : 'a) => (mass d a) 
          sum (fun (b : 'b) => if M b then  mass (f a) b else 0%r)).
 apply fun_ext. move => a.
 have ooo : mu (f a) M = sum (fun (b0 : 'b) => if M b0 then mass (f a) b0 else 0%r).
-apply muE.
-smt.
-rewrite qqq.
-rewrite (dletE_swap' d f M). auto.
+rewrite muE.
+smt(massE).
+smt(massE).
+rewrite  (dletE_swap' d f M). rewrite qqq. auto.
 qed.
 
 
 lemma all_distr_countable (X : 'a distr) : countable (support X). 
 proof. rewrite /support.  
-  have ->: (fun (x : 'a) => 0%r < mu1 X x) 
-         = (fun (x : 'a) => 0%r < mass X x).
-   apply fun_ext.  move=> x. rewrite massE. auto.
-  have ->: (fun (x : 'a) => 0%r < mass X x)
-         = (fun (x : 'a) => mass X x <> 0%r).
-    apply fun_ext.  move => x. smt.
-apply (countable_mass X).
+  have ->: (fun (x : 'a) => 0%r < mu1 X x)
+         = (fun (x : 'a) => mu1 X x <> 0%r).
+    apply fun_ext.  move => x. smt(massE @Distr).
+apply (countable_mu1 X).
 qed.
 
 
 lemma dmeq ['a, 'b] (d : 'a distr) (M : 'b * 'a -> bool) (r : 'b) : 
    mu d (fun x => M (r, x)) = mu (dmap d (fun x => (r, x))) M.
-proof. rewrite dmapE. simplify. smt. 
+proof. rewrite dmapE. simplify. smt(). 
 qed.
 
 
 lemma zkj ['a] f : forall x (l : 'a list),
   big predT f (x :: l) = (f x) + big predT f l.
-proof. smt.
+proof. smt().
 qed.
 
 
 lemma sm_than (a b : real) : (forall e, e > 0%r => a >= b - e) => a >= b.
 proof. case (b <= a). auto.
 move => asbn.
-have : a < b. smt.
+have : a < b. smt().
 move => asb pr. clear asbn.
 pose d := b - a.
-have : d > 0%r. smt.
+have : d > 0%r. smt().
 move => dpos.
-have : d = b - a. smt.
+have : d = b - a. smt().
 move => deq.
-have : exists q, q > 0%r /\ q < d. smt.
+have : exists q, q > 0%r /\ q < d. smt().
 elim. move => q [qp1] qp2. 
-have : d - q > 0%r. smt.
+have : d - q > 0%r. smt().
 move => dmq.
-have : b - (d - q) <= a. smt.
-smt.
+have : b - (d - q) <= a. smt().
+smt().
 qed.
 
 
@@ -109,11 +107,11 @@ lemma jokk ['a] (d1 d2 : 'a distr) :
   (forall M, mu d1 M <= mu d2 M) 
   => forall J, enumerate J (support d2) => enumerate J (support d1).
 move => pr. move => j ejd2. 
-split. smt.
+split. smt().
 move => x xid1.   
 elim ejd2. move => q1 q2.
 apply (q2 x).
-smt.
+smt().
 qed.
 
 
@@ -121,7 +119,7 @@ lemma prjokk ['a]  (d  : 'a distr) j J :
   enumerate J (support d) => enumerate j (support d)
   => forall n, exists N, forall x, x \in d => x \in (pmap j (range 0 n)) 
       => x \in (pmap J (range 0 N)).
-move => e1 e2.  apply natind. smt.
+move => e1 e2.  apply natind. smt(@List).
 simplify. move => n nc ih. 
 elim ih. move => N Np.
 case (j n = None).
@@ -130,32 +128,32 @@ have : forall m, j m = None => pmap j (range 0 (m+1)) = pmap j (range 0 m).
 apply natind.  simplify.
 move => n0 n0p zz. 
 case (n0 < 0).
-smt.
+smt(@List).
 move => nlz.
-have : n0 = 0. smt. 
+have : n0 = 0. smt(). 
 move => ko. rewrite ko. simplify.
    simplify pmap.
-have : pmap j (range 0 0) = []. smt.
+have : pmap j (range 0 0) = []. smt(@List).
 move => ke. rewrite ke. clear ke.
-have : range 0 1 = 0 :: []. smt.
-move => ke. rewrite ke. clear ke. simplify.  smt.
+have : range 0 1 = 0 :: []. smt(@List).
+move => ke. rewrite ke. clear ke. simplify. smt().
 simplify.
 move => n0 n0p. move => ih2 pr.
-rewrite (rangeSr 0 (n0+1)) . smt.
+rewrite (rangeSr 0 (n0+1)) . smt().
 rewrite - cats1.
 rewrite pmap_cat. 
 have : pmap j [n0 + 1] = [].
-smt.
-move => k. rewrite k. smt.
+smt(@List).
+move => k. rewrite k. smt(@List).
 move => prop. exists N. move => x. rewrite prop. auto. progress. apply Np. auto. auto.
 move => jnn.
 pose z := (j n).
-have : z = (j n). smt. 
-have : z <> None. smt.
+have : z = (j n). smt(). 
+have : z <> None. smt().
 elim (j n).
- smt.
+ smt().
 move => a ap1 ap2.
-have : j n = Some a. smt.
+have : j n = Some a. smt().
 move => q.
 elim e1.
 move => q1 q2.
@@ -164,59 +162,59 @@ move => aid.
 elim (q2 a aid). move => i ip. 
 case (i < N).
 move => inp. exists N.
-move => x xd. rewrite rangeSr. smt. rewrite - cats1. rewrite pmap_cat.
+move => x xd. rewrite rangeSr. smt(). rewrite - cats1. rewrite pmap_cat.
 case (x \in pmap j (range 0 n)).
 move => xn. move => _. apply Np. auto. auto.
 move => alt alt2.
-have : x = a. smt.
+have : x = a. smt(@List).
 move => xa. rewrite xa. clear alt alt2. clear Np. 
-have : i \in (range 0 N). apply mem_range. smt. smt.
+have : i \in (range 0 N). apply mem_range. smt(). smt(@List).
 move => npr.
-have : N <= i.  smt.
+have : N <= i.  smt().
 clear npr. move => npr.
 exists (i+1).
-move => x xd. rewrite rangeSr. smt. rewrite - cats1. rewrite pmap_cat.
+move => x xd. rewrite rangeSr. smt(). rewrite - cats1. rewrite pmap_cat.
 have qq : forall x (n : int) m, n <= m => x \in pmap J (range 0 n) => x \in pmap J (range 0 m).
 move => xx nn mm nm xip.
 elim (pmapP J (range 0 nn) xx ).
 move => ok1 ok2. elim (ok1 xip). move => x0. elim. move => x01 x02. 
-have : x0 \in (range 0 mm). smt.
-smt.
+have : x0 \in (range 0 mm). smt(@List).
+smt(@List).
 case (x \in pmap j (range 0 n)).
 move => l1 l2.
-apply (qq x N (i+1)). smt.
+apply (qq x N (i+1)). smt().
 apply Np. auto. auto.
 move => alt alt2.
-have : x = a. smt.
+have : x = a. smt(@List).
 move => xa. rewrite xa.
-have : i  \in (range 0 (i+1)). smt. smt.
+have : i  \in (range 0 (i+1)). smt(@List). smt(@List).
 move => anid.
 exists N.
 move => x xd.
-rewrite rangeSr. smt. rewrite - cats1. rewrite pmap_cat.
+rewrite rangeSr. smt(). rewrite - cats1. rewrite pmap_cat.
 case (x \in pmap j (range 0 n)).
 move => xn. move => _. apply Np. auto. auto.
 move => alt alt2.
-have : x = a. smt.
-smt.
+have : x = a. smt(@List).
+smt().
 qed.
 
 
-lemma abs1 : forall (a c : real) , `|a * c| = `|a| * `|c|. by smt. qed. 
+lemma abs1 : forall (a c : real) , `|a * c| = `|a| * `|c|. by smt(). qed. 
 
 
-lemma abs2 : forall (a : real) ,  a >= 0%r =>  `|a| = a. by smt. qed.
+lemma abs2 : forall (a : real) ,  a >= 0%r =>  `|a| = a. by smt(). qed.
 
 
-lemma abs3 : forall (a : real), `|a| >= 0%r. by smt. qed.
+lemma abs3 : forall (a : real), `|a| >= 0%r. by smt(). qed.
 
 
 lemma pmc1 (N : int)  : forall  m (x : int), N <= m => x \in (range 0 N) 
-  => x \in (range 0 m). by smt. qed.
+  => x \in (range 0 m). by smt(@List). qed.
 
 
 lemma pmc2 ['a] J    : forall  l m (x : 'a), (forall (y : int), mem  l y => mem m y) 
-  => x \in pmap J l => x \in pmap J m. by smt. qed.
+  => x \in pmap J l => x \in pmap J m. by smt(@List). qed.
 
 
 lemma pmc ['a] J (N : int)  : forall  m (x : 'a), N <= m => x \in pmap J (range 0 N) 
